Add par subst

theories/semtyping.v
@@ -1,39 +1,27 @@
 Require Import Autosubst2.syntax unscoped par typing.
+Require Import FunctionalExtensionality PropExtensionality.
+From stdpp Require Import relations (rtc(..)).
 Require Import ssreflect.
 From Hammer Require Import Tactics.
+From Equations Require Import Equations.
 
 Definition ProdSpace (PA : Tm -> Prop) (PF : Tm -> (Tm -> Prop) -> Prop) (b : Tm) :=
   forall a PB, PA a -> PF a PB -> PB (App b a).
 
-Definition ProdSpaceS (PA : Tm -> Prop) (PF : Tm -> Prop -> Prop) :=
-  forall a P, PA a -> PF a P -> P.
-
-(* Candidate : (Ty -> Prop) -> Prop *)
-
-(* P in Candidate iff *)
-
-(* let Box x = a in b *)
-
-(* InterpExists A : exists i S, Interp i A S /\ exists a, S a. *)
-
-
-(* How does I affect the inhabitance? *)
 Inductive InterpExt i I : Tm -> (Tm -> Prop) -> Prop :=
+| InterpExt_Ne A
 | InterpExt_Fun A B PA PF :
   InterpExt i I A PA ->
   (forall a, PA a -> exists PB, PF a PB) ->
   (forall a PB, PA a -> PF a PB -> InterpExt i I (subst_Tm (scons a ids) B) PB) ->
   InterpExt i I (Pi A B) (ProdSpace PA PF)
 
-(* TODO *)
-(* Try using candidates to capture the definition of InterpExtSquashed? *)
-| InterpExt_Squash j A  P :
-  (* Latest thoughts: *)
-  (* What if we don't pass in I but something else that's more generic? *)
-  (* What can we say in terms of inhabitance? *)
-  InterpExt j I A P ->
+| InterpExt_Squash A :
   (* -------------------- *)
-  InterpExt i I (Squash A) P
+  InterpExt i I (Squash A) (fun a => exists b, rtc Par a (Box b))
+
+| InterpExt_Empty :
+  InterpExt i I Empty (fun a => False)
 
 | InterpExt_Univ j :
   j < i ->
@@ -44,42 +32,77 @@ Inductive InterpExt i I : Tm -> (Tm -> Prop) -> Prop :=
   InterpExt i I A0 PA ->
   InterpExt i I A PA.
 
-Lemma InterpExt_same_inhab i I0 I1 A S0 S1 :
-  InterpExt i I0 A S0 ->
-  InterpExt i I1 A S1 ->
-  ((exists a, S0 a) <-> (exists a, S1 a)).
+Equations InterpUnivN (i : nat) : Tm -> (Tm -> Prop) -> Prop
+  by wf i lt :=
+  InterpUnivN i := InterpExt i
+                       (fun j A =>
+                          match Compare_dec.lt_dec j i with
+                          | left h => exists PA, InterpUnivN j A PA
+                          | right _ => False
+                          end).
+
+Lemma InterpExt_Univ' i I j PF :
+  PF = (fun A => I j A) ->
+  j < i ->
+  InterpExt i I (Univ j) PF.
+Proof. hauto lq:on ctrs:InterpExt. Qed.
+
+Lemma InterpExt_lt_redundant i I0 I1 A PA
+  (h0 : forall j,  j < i -> I0 j = I1 j)
+  (h : InterpExt i I0 A PA) :
+       InterpExt i I1 A PA.
 Proof.
-  move => h. move : I1 S1.
-  elim : i I0 A S0 / h.
-  - move => i I0 A B PA PF hPA ihPA hTot hRes ihPF I1 S1.
+  elim : A PA / h.
+  - hauto lq:on ctrs:InterpExt.
+  - hauto l:on.
+  - hauto l:on ctrs:InterpExt.
+  - hauto lq:on use:InterpExt_Univ.
+  - hauto l:on ctrs:InterpExt.
+Qed.
+
+Lemma InterpExt_lt_redundant_iff i I0 I1 A PA
+  (h0 : forall j,  j < i -> I0 j = I1 j) :
+  (InterpExt i I0 A PA <-> InterpExt i I1 A PA).
+Proof.
+  have : forall j : nat, j < i -> I1 j = I0 j by firstorder.
+  firstorder using InterpExt_lt_redundant.
+Qed.
+
+Lemma InterpUnivN_nolt i :
+  InterpUnivN i = InterpExt i (fun j A => exists PA, InterpUnivN j A PA).
+Proof.
+  simp InterpUnivN.
+  extensionality A.
+  extensionality S.
+  apply propositional_extensionality.
+  apply InterpExt_lt_redundant_iff.
+  move => j ?.
+  case : Compare_dec.lt_dec=>//=.
+Qed.
+
+#[export]Hint Rewrite InterpUnivN_nolt : InterpUniv.
+
+Lemma InterpExt_Fun_inv i I A B P
+  (h :  InterpExt i I (Pi A B) P) :
+  exists PA PF,
+    InterpExt i I A PA /\
+    (forall a, PA a -> exists PB, PF a PB) /\
+    (forall a PB, PA a -> PF a PB -> InterpExt i I (subst_Tm (scons a ids) B) PB) /\
+    P = ProdSpace PA PF.
+Proof.
+  move E : (Pi A B) h => T h.
+  move : A B E.
+  elim : T P / h => //.
+  - hauto l:on.
+  - move => *. subst.
     admit.
-  - admit.
-  - admit.
-  -
-(* Idea: the contravariance of function arguments might matter less if
-the entire thing is a proposition (we only care about whether the
-output is inhabited). In other words,   *)
-with InterpExtSquashed I : Tm -> Prop -> Prop :=
-| InterpExtS_Fun i A B PA (PF : Tm -> Prop -> Prop) :
-  InterpExt i I A PA ->
-  (forall a, PA a -> exists PB, PF a PB) ->
-  (forall a PB, PA a -> PF a PB -> InterpExtSquashed I (subst_Tm (scons a ids) B) PB) ->
-  InterpExtSquashed I (Pi A B) (ProdSpaceS PA PF)
-
-| InterpExtS_Univ j :
-  InterpExtSquashed I (Univ j) True
-
-| InterpExtS_Squash A P :
-  InterpExtSquashed I A P ->
-  InterpExtSquashed I (Squash A) P
-
-| InterpExtS_Step A A0 PA :
-  A ⇒ A0 ->
-  InterpExtSquashed I A0 PA ->
-  InterpExtSquashed I A PA.
+Admitted.
 
 
+Definition ρ_ok Γ := forall i ℓ A,
+    Lookup i Γ ℓ A ->
+    match ℓ with
+    | Irrel => True
+    | Rel => forall m PA, InterpUnivN .
 
-(* Define another InterpExtProp function that treats the codomains as squashed? *)
-(* InterpExtProp: defined in terms of InterpExt *)
-(* InterpExt: characterizes InterpExtProp with axioms *)
+IOk (c2e Δ) ℓ (ρ i) /\ forall m PA, ⟦ c2e Δ ⊨ A [ρ] ⟧ m ↘ PA -> PA ℓ (ρ i).
