theories/par.v
@@ -1,5 +1,8 @@
-Require Import Autosubst2.syntax unscoped FunInd.
+Require Import Autosubst2.syntax unscoped core FunInd ssreflect.
+From Hammer Require Import Tactics.
 From stdpp Require Import relations (rtc(..)).
+
+Variant Level := Rel | Irrel.
 
 Reserved Infix "⇒" (at level 60, right associativity).
 Inductive Par : Tm -> Tm -> Prop :=
@@ -54,5 +57,74 @@ Inductive Par : Tm -> Tm -> Prop :=
   (* ------------------- *)
   Absurd a0 ⇒ Absurd a1
 where "A ⇒ B" := (Par A B).
+#[export]Hint Constructors Par : par.
 
 Definition Coherent A B := exists C, rtc Par A C /\ rtc Par B C.
+
+Derive Inversion Par_inv with (forall a b, a ⇒ b).
+
+Lemma Par_refl a : a ⇒ a.
+Proof. elim : a; hauto lq:on ctrs:Par. Qed.
+
+Lemma P_AppAbs_cbn a b b0 :
+  b0 = subst_Tm (scons b ids) a ->
+  (App (Abs a) b) ⇒ b0.
+Proof. hauto lq:on ctrs:Par use:Par_refl. Qed.
+
+Lemma P_AppAbs' a a0 b0 b1 b:
+  b = subst_Tm (scons b1 ids) a0 ->
+  a ⇒ a0 ->
+  b0 ⇒ b1 ->
+  (* ---------------------------- *)
+  App (Abs a) b0 ⇒ b.
+Proof. hauto lq:on use:P_AppAbs. Qed.
+
+Lemma P_LetBox' a0 a1 b0 b1 b :
+  b = subst_Tm (scons a1 ids) b1 ->
+  a0 ⇒ a1 ->
+  b0 ⇒ b1 ->
+  (* ------------------------- *)
+  Let (Box a0) b0 ⇒ b.
+Proof. hauto lq:on use:P_LetBox. Qed.
+
+Lemma Par_renaming a b ξ :
+  a ⇒ b -> ren_Tm ξ a ⇒ ren_Tm ξ b.
+Proof.
+  move => h.
+  move : ξ.
+  elim : a b / h => /=; eauto with par.
+  - move => *.
+    apply : P_AppAbs'; eauto. by asimpl.
+  - move => *.
+    apply : P_LetBox'; eauto; by asimpl.
+Qed.
+
+Lemma Par_morphing_lift (ξ0 ξ1 : nat -> Tm)
+  (h : forall i, (ξ0 i ⇒ ξ1 i)) :
+  forall i, (up_Tm_Tm ξ0 i ⇒ up_Tm_Tm ξ1 i).
+Proof. qauto l:on inv:nat use:Par_refl, Par_renaming. Qed.
+
+Lemma Par_morphing a b σ0 σ1
+  (h : forall i, σ0 i ⇒ σ1 i) :
+  (a ⇒ b) ->
+  (subst_Tm σ0 a ⇒ subst_Tm σ1 b).
+Proof.
+  move => h0.
+  move : σ0 σ1 h.
+  elim : a b/h0; try solve [move => //=; eauto with par].
+  - hauto lq:on ctrs:Par use:Par_morphing_lift.
+  - hauto lq:on ctrs:Par use:Par_morphing_lift.
+  - move => a a0 b0 b1 h0 ih0 h1 ih1 σ0 σ h /=.
+    apply : P_AppAbs'; cycle 1; eauto.
+    sfirstorder use:Par_morphing_lift.
+    by asimpl.
+  - hauto lq:on ctrs:Par use:Par_morphing_lift.
+  - move => * /=.
+    apply : P_LetBox'; cycle 1; eauto.
+    sfirstorder use:Par_morphing_lift.
+    by asimpl.
+Qed.
+
+Lemma Par_subst a0 a1 (h : a0 ⇒ a1) σ :
+  (subst_Tm σ a0 ⇒ subst_Tm σ a1).
+Proof. hauto l:on use:Par_refl, Par_morphing. Qed.
